型制約を書き始めた

TypeSubst.v
@@ -3,31 +3,31 @@ Require Import String.
 Require Import Term.
 Require Import Typing.
 
-Definition ctx := tenv.
-Module Ctx := TEnv.
+Definition tsubst := tenv.
+Module Tsubst := TEnv.
 
-Inductive TypeSubst : type -> type -> ctx -> Prop :=
-  SVarT1 : forall ctx x T, Ctx.MapsTo x T ctx -> TypeSubst (VarT x) T ctx
-| SVarT2 : forall ctx x, ~ Ctx.In x ctx -> TypeSubst (VarT x) (VarT x) ctx
-| SBoolT : forall ctx    , TypeSubst BoolT BoolT ctx
-| SFunT  : forall ctx T1 T2 S1 S2 ,
-    TypeSubst T1 S1 ctx -> TypeSubst T2 S2 ctx -> TypeSubst (FunT T1 T2) (FunT S1 S2) ctx.
+Inductive TypeSubst : type -> type -> tsubst -> Prop :=
+  SVarT1 : forall tsubst x T, Tsubst.MapsTo x T tsubst -> TypeSubst (VarT x) T tsubst
+| SVarT2 : forall tsubst x, ~ Tsubst.In x tsubst -> TypeSubst (VarT x) (VarT x) tsubst
+| SBoolT : forall tsubst    , TypeSubst BoolT BoolT tsubst
+| SFunT  : forall tsubst T1 T2 S1 S2 ,
+    TypeSubst T1 S1 tsubst -> TypeSubst T2 S2 tsubst -> TypeSubst (FunT T1 T2) (FunT S1 S2) tsubst.
 
-Definition TEnvSubst (tenv1 tenv2 : tenv) (ctx : ctx):= forall x T S,
-  TEnv.MapsTo x T tenv1 -> TypeSubst T S ctx -> TEnv.MapsTo x S tenv2.
+Definition TEnvSubst (tenv1 tenv2 : tenv) (tsubst : tsubst):= forall x T S,
+  TEnv.MapsTo x T tenv1 -> TypeSubst T S tsubst -> TEnv.MapsTo x S tenv2.
 
-Inductive TermSubst : term -> term -> ctx -> Prop :=
-   SVar  : forall ctx x, TermSubst (Var x) (Var x) ctx
- | SBool : forall ctx b, TermSubst (Bool b) (Bool b) ctx
- | SLambda : forall ctx x T S t s, TypeSubst T S ctx -> TermSubst t s ctx ->
-              TermSubst (Lambda x T t) (Lambda x S s) ctx
- | SApply : forall ctx t1 t2 s1 s2,       TermSubst t1 s1 ctx -> TermSubst t2 s2 ctx ->
-              TermSubst (Apply t1 t2) (Apply s1 s2) ctx
- | SIf    : forall ctx t1 t2 t3 s1 s2 s3, TermSubst t1 s1 ctx -> TermSubst t2 s2 ctx -> TermSubst t3 s3 ctx ->
-              TermSubst (If t1 t2 t3) (If s1 s2 s3) ctx.
+Inductive TermSubst : term -> term -> tsubst -> Prop :=
+   SVar  : forall tsubst x, TermSubst (Var x) (Var x) tsubst
+ | SBool : forall tsubst b, TermSubst (Bool b) (Bool b) tsubst
+ | SLambda : forall tsubst x T S t s, TypeSubst T S tsubst -> TermSubst t s tsubst ->
+              TermSubst (Lambda x T t) (Lambda x S s) tsubst
+ | SApply : forall tsubst t1 t2 s1 s2,       TermSubst t1 s1 tsubst -> TermSubst t2 s2 tsubst ->
+              TermSubst (Apply t1 t2) (Apply s1 s2) tsubst
+ | SIf    : forall tsubst t1 t2 t3 s1 s2 s3, TermSubst t1 s1 tsubst -> TermSubst t2 s2 tsubst -> TermSubst t3 s3 tsubst ->
+              TermSubst (If t1 t2 t3) (If s1 s2 s3) tsubst.
 
-Lemma MapsTo_In : forall (A : Type) (ctx : TEnv.t A) x (T : A),
-  TEnv.MapsTo x T ctx -> TEnv.In x ctx.
+Lemma MapsTo_In : forall (A : Type) (tsubst : TEnv.t A) x (T : A),
+  TEnv.MapsTo x T tsubst -> TEnv.In x tsubst.
 Proof.
 intros.
 unfold TEnv.In in |- *.
@@ -37,13 +37,13 @@ exists T.
 exact H.
 Qed.
 
-Lemma subst_uniq : forall ctx T S U,
-  TypeSubst T S ctx -> TypeSubst T U ctx -> S = U.
+Lemma subst_uniq : forall tsubst T S U,
+  TypeSubst T S tsubst -> TypeSubst T U tsubst -> S = U.
 Proof.
 induction T.
  intros.
  inversion H; inversion H0.
-  apply TEnvWF.MapsTo_fun with (m := ctx0) (x := s).
+  apply TEnvWF.MapsTo_fun with (m := tsubst0) (x := s).
    exact H2.
 
    exact H6.
@@ -78,10 +78,10 @@ induction T.
    reflexivity.
 Qed.
 
-Lemma subst_add : forall ctx tenv1 tenv2 x S T,
-   TEnvSubst tenv1 tenv2 ctx ->
-   TypeSubst S T ctx ->
-   TEnvSubst (TEnv.add x S tenv1) (TEnv.add x T tenv2) ctx.
+Lemma subst_add : forall tsubst tenv1 tenv2 x S T,
+   TEnvSubst tenv1 tenv2 tsubst ->
+   TypeSubst S T tsubst ->
+   TEnvSubst (TEnv.add x S tenv1) (TEnv.add x T tenv2) tsubst.
 Proof.
 intros.
 unfold TEnvSubst in |- *.
@@ -92,7 +92,7 @@ inversion H1.
  rewrite <- H5 in H2.
  rewrite <- H4 in |- *.
  assert (S0 = T).
-  apply subst_uniq with (T := S) (ctx := ctx0).
+  apply subst_uniq with (T := S) (tsubst := tsubst0).
    exact H2.
 
    exact H0.
@@ -112,12 +112,12 @@ inversion H1.
    exact H2.
 Qed.
 
-Lemma subst_exists : forall T ctx,
-   exists S, TypeSubst T S ctx.
+Lemma subst_exists : forall T tsubst,
+   exists S, TypeSubst T S tsubst.
 Proof.
 intros.
 induction T.
- destruct (TEnvWF.In_dec ctx0 s).
+ destruct (TEnvWF.In_dec tsubst0 s).
   inversion i.
   exists x.
   apply SVarT1.
@@ -140,13 +140,13 @@ induction T.
   exact H0.
 Qed.
 
-Theorem subst_preserve : forall ctx s tenv2 S t tenv1 T,
-  Typed t tenv1 T -> (TEnvSubst tenv1 tenv2 ctx -> TermSubst t s ctx -> TypeSubst T S ctx ->
+Theorem subst_preserve : forall tsubst s tenv2 S t tenv1 T,
+  Typed t tenv1 T -> (TEnvSubst tenv1 tenv2 tsubst -> TermSubst t s tsubst -> TypeSubst T S tsubst ->
   Typed s tenv2 S).
 Proof.
 intros until T.
 intro.
-generalize ctx0, s, tenv2, S.
+generalize tsubst0, s, tenv2, S.
 pattern t, tenv1, T in |- *.
 apply Typed_ind.
  intros.
@@ -167,14 +167,14 @@ apply Typed_ind.
  inversion H3.
  inversion H4.
  assert (S1 = S2).
-  apply subst_uniq with (ctx := ctx1) (T := a).
+  apply subst_uniq with (tsubst := tsubst1) (T := a).
    exact H10.
 
    exact H14.
 
   rewrite H18 in |- *.
   apply TLambda.
-  apply H1 with (ctx0 := ctx1).
+  apply H1 with (tsubst0 := tsubst1).
    apply subst_add.
     exact H2.
 
@@ -186,12 +186,12 @@ apply Typed_ind.
 
  intros.
  inversion H5.
- assert (exists T : type, TypeSubst a T ctx1).
+ assert (exists T : type, TypeSubst a T tsubst1).
   apply subst_exists.
 
   decompose [ex] H13.
   apply TApply with (a := x).
-   apply H1 with (ctx0 := ctx1).
+   apply H1 with (tsubst0 := tsubst1).
     exact H4.
 
     exact H9.
@@ -201,7 +201,7 @@ apply Typed_ind.
 
      exact H6.
 
-   apply H3 with (ctx0 := ctx1).
+   apply H3 with (tsubst0 := tsubst1).
     exact H4.
 
     exact H12.
@@ -211,21 +211,21 @@ apply Typed_ind.
  intros.
  inversion H7.
  apply TIf.
-  apply H1 with (ctx0 := ctx1).
+  apply H1 with (tsubst0 := tsubst1).
    exact H6.
 
    exact H12.
 
    apply SBoolT.
 
-  apply H3 with (ctx0 := ctx1).
+  apply H3 with (tsubst0 := tsubst1).
    exact H6.
 
    exact H15.
 
    exact H8.
 
-  apply H5 with (ctx0 := ctx1).
+  apply H5 with (tsubst0 := tsubst1).
    exact H6.
 
    exact H16.
