Constraint.v
@@ -1,0 +1,7 @@
+Require Import List.
+Require Import Term.
+Require Import TypeSubst.
+
+Definition constraints := list (type * type).
+Definition Unified (c : constraints) (t : tsubst) := forall S T U,
+  In (S,T) c -> TypeSubst S U t /\ TypeSubst T U t.
